src/Pipit.Exp.Checked.Subst.fst
@@ -1,0 +1,366 @@
+(* Properties about checked semantics and substitution *)
+module Pipit.Exp.Checked.Subst
+
+open Pipit.Exp.Checked.Base
+
+open Pipit.Prim.Table
+
+open Pipit.Exp.Base
+open Pipit.Exp.Bigstep
+open Pipit.Exp.Binding
+open Pipit.Exp.Binding.Properties
+
+open Pipit.Exp.Causality
+
+module C  = Pipit.Context.Base
+module CP = Pipit.Context.Properties
+module PM = Pipit.Prop.Metadata
+
+module List = FStar.List.Tot
+
+open FStar.Squash
+
+#push-options "--split_queries always"
+
+let subst_extend_dropped
+  (#t: table)
+  (#c: context t)
+  (i: C.index_lookup c)
+  (rows: list (row (C.drop1 c i)))
+  (e: exp t (C.drop1 c i) (C.get_index c i) { causal e }):
+    Tot (r': (list (row c)) { List.length r' == List.length rows }) =
+  CP.row_zip2_lift1_dropped i rows (lemma_bigsteps_total_vs rows e)
+
+let rec lemma_bigstep_always_substitute
+  (#t: table)
+  (#c: context t)
+  (i: C.index_lookup c)
+  (rows: list (row (C.drop1 c i)))
+  (e: exp t (C.drop1 c i) (C.get_index c i) { causal e })
+  (e': exp t c t.propty):
+  Lemma (ensures (
+    bigstep_always rows (subst1' e' i e) <==>
+    bigstep_always (subst_extend_dropped i rows e) e'
+  )) =
+  match rows with
+  | [] -> ()
+  | r::rows' ->
+    // TODO:ADMIT: squash, apply lemma_bigstep_substitute_elim, intros
+    assume (bigstep rows (subst1' e' i e) true <==>
+    bigstep (subst_extend_dropped i rows e) e' true);
+    lemma_bigstep_always_substitute i rows' e e'
+
+let rec lemma_check_substitute_elim
+  (#t: table)
+  (#c: context t)
+  (#a: t.ty)
+  (mode: PM.check_mode)
+  (i: C.index_lookup c)
+  (rows: list (row (C.drop1 c i)) { Cons? rows })
+  (e: exp t (C.drop1 c i) (C.get_index c i) { causal e })
+  (e': exp t c a)
+  (hCKe': check mode rows (subst1' e' i e)):
+    Tot (check mode (subst_extend_dropped i rows e) e') (decreases hCKe') =
+  let rows' = subst_extend_dropped i rows e in
+  match e' with
+  | XBase b -> CkBase _ b
+  | XApps ea ->
+    let CkApps _ _ hCKa = hCKe' in
+    CkApps _ _ (lemma_check_substitute_elim_apps mode i rows e ea hCKa)
+  | XFby v1 e2 ->
+    (match hCKe' with
+    | CkFby1 _ _ _ -> CkFby1 rows' v1 e2
+    | CkFbyS _ _ _ _ hCK2 ->
+      CkFbyS (List.hd rows') (List.tl rows') v1 e2 (lemma_check_substitute_elim mode i (List.tl rows) e e2 hCK2))
+
+  | XMu e1 ->
+    let CkMu _ _ hCK1 = hCKe' in
+    lemma_subst_subst_distribute_XMu e1 i e;
+    let hCK1' = lemma_check_substitute_elim mode i rows e (subst1 e1 (XMu e1)) hCK1 in
+    CkMu _ e1 hCK1'
+
+  | XLet b e1 e2 ->
+    let CkLet _ _ _ hCK = hCKe' in
+    lemma_subst_subst_distribute_le e2 0 i e1 e;
+    let hCK' = lemma_check_substitute_elim mode i rows e (subst1 e2 e1) hCK in
+    CkLet _ e1 e2 hCK'
+
+  | XCheck ps e1 ->
+    let CkCheck _ _ _ hCK hBS = hCKe' in
+    let hCK' = lemma_check_substitute_elim mode i rows e e1 hCK in
+    lemma_bigstep_always_substitute i rows e e1;
+    CkCheck _ ps e1 hCK' ()
+
+  | XContract ps er eg eb ->
+    let CkContract _ _ _ _ _ hTr hTrg hCr hCgb = hCKe' in
+    lemma_bigstep_always_substitute i rows e er;
+    lemma_bigstep_always_substitute i rows e (subst1 eg eb);
+
+    let hTr' = () in
+    let hTrg' = () in
+
+    let hCr' = lemma_check_substitute_elim mode i rows e er hCr in
+
+    let hCgb' = match hCgb with
+      | Inl hN ->
+        Inl ()
+      | Inr (hCb,hCg) ->
+        lemma_subst_subst_distribute_le eg 0 i eb e;
+        let hCb' = lemma_check_substitute_elim mode i rows e eb hCb in
+        let hCg' = lemma_check_substitute_elim mode i rows e (subst1 eg eb) hCg in
+        Inr (hCb', hCg')
+    in
+
+    CkContract _ ps er eg eb hTr' hTrg' hCr' hCgb'
+
+and lemma_check_substitute_elim_apps
+  (#t: table)
+  (#c: context t)
+  (#a: funty t.ty)
+  (mode: PM.check_mode)
+  (i: C.index_lookup c)
+  (rows: list (row (C.drop1 c i)) { Cons? rows })
+  (e: exp t (C.drop1 c i) (C.get_index c i) { causal e })
+  (e': exp_apps t c a)
+  (hCKe': check_apps mode rows (subst1_apps' e' i e)):
+    Tot (check_apps mode (subst_extend_dropped i rows e) e') (decreases hCKe') =
+  let rows' = subst_extend_dropped i rows e in
+  match e' with
+  | XPrim f -> CkPrim rows' f
+  | XApp ef ea ->
+    let CkApp _ _ _ hCKf hCKa = hCKe' in
+    let hCKf' = lemma_check_substitute_elim_apps mode i rows e ef hCKf in
+    let hCKa' = lemma_check_substitute_elim mode i rows e ea hCKa in
+    CkApp rows' _ _ hCKf' hCKa'
+
+
+let lemma_check_substitute_intros_base
+  (#t: table)
+  (#c: context t)
+  (#a: t.ty)
+  (mode: PM.check_mode)
+  (i: C.index_lookup c)
+  (rows: list (row (C.drop1 c i)))
+  (e: exp t (C.drop1 c i) (C.get_index c i) { causal e })
+  (e': exp_base t c a)
+  (hCKe: check mode rows e):
+    Tot (check mode rows (subst1_base' e' i e)) =
+  match e' with
+  | XVal v -> CkBase rows (XVal v)
+  | XVar x -> CkBase rows (XVar x)
+  | XBVar i' ->
+    if i = i'
+    then hCKe
+    else if i' < i
+    then (
+      CP.lemma_drop_get_index_lt c i i';
+      let i': C.index_lookup (C.drop1 c i) = i' in
+      let xv: exp_base t (C.drop1 c i) a = XBVar i' in
+      CkBase rows xv
+    ) else (
+      CP.lemma_drop_get_index_gt c i (i' - 1);
+      assert (C.opt_index (C.drop1 c i) (i' - 1) == Some (C.get_index c i'));
+      assert_norm (subst1_base' (XBVar i') i e == XBase (XBVar #t #(C.drop1 c i) (i' - 1)));
+      CkBase rows (XBVar (i' - 1)))
+
+let rec lemma_check_substitute_intros
+  (#t: table)
+  (#c: context t)
+  (#a: t.ty)
+  (mode: PM.check_mode)
+  (i: C.index_lookup c)
+  (rows: list (row (C.drop1 c i)))
+  (e: exp t (C.drop1 c i) (C.get_index c i) { causal e })
+  (e': exp t c a)
+  (hCKe: (r: list (row (C.drop1 c i)) { List.length r <= List.length rows }) -> check mode r e)
+  (hCKe': check mode (subst_extend_dropped i rows e) e'):
+    Tot (check mode rows (subst1' e' i e)) (decreases hCKe') =
+  match e' with
+  | XBase b ->
+    lemma_check_substitute_intros_base mode i rows e b (hCKe rows)
+
+  | XApps ea ->
+    let CkApps _ _ hCKa = hCKe' in
+    CkApps _ _ (lemma_check_substitute_intros_apps mode i rows e ea hCKe hCKa)
+
+  | XFby v1 e2 ->
+    (match hCKe' with
+    | CkFby1 _ _ _ -> CkFby1 rows v1 (subst1' e2 i e)
+    | CkFbyS _ _ _ _ hCK2 ->
+      CkFbyS (List.hd rows) (List.tl rows) v1 (subst1' e2 i e) (lemma_check_substitute_intros mode i (List.tl rows) e e2 hCKe hCK2))
+
+  | XMu e1 ->
+    let CkMu _ _ hCK1 = hCKe' in
+    lemma_subst_subst_distribute_XMu e1 i e;
+    let hCK1' = lemma_check_substitute_intros mode i rows e (subst1 e1 (XMu e1)) hCKe hCK1 in
+    CkMu _ (subst1' e1 (i + 1) (lift1 e a)) hCK1'
+
+  | XLet b e1 e2 ->
+    let CkLet _ _ _ hCK = hCKe' in
+    lemma_subst_subst_distribute_le e2 0 i e1 e;
+    let hCK' = lemma_check_substitute_intros mode i rows e (subst1 e2 e1) hCKe hCK in
+    CkLet _ (subst1' e1 i e) (subst1' e2 (i + 1) (lift1 e b)) hCK'
+
+  | XCheck ps e1 ->
+    let CkCheck _ _ _ hCK hBS = hCKe' in
+    let hCK' = lemma_check_substitute_intros mode i rows e e1 hCKe hCK in
+    lemma_bigstep_always_substitute i rows e e1;
+    CkCheck _ ps (subst1' e1 i e) hCK' ()
+
+  | XContract ps er eg eb ->
+    let CkContract _ _ _ _ _ hTr hTrg hCr hCgb = hCKe' in
+    lemma_bigstep_always_substitute i rows e er;
+    lemma_bigstep_always_substitute i rows e (subst1 eg eb);
+
+    let hTr' = () in
+    let hTrg' = () in
+
+    let hCr' = lemma_check_substitute_intros mode i rows e er hCKe hCr in
+
+    let hCgb' = match hCgb with
+      | Inl hN ->
+        Inl ()
+      | Inr (hCb,hCg) ->
+        lemma_subst_subst_distribute_le eg 0 i eb e;
+        let hCb' = lemma_check_substitute_intros mode i rows e eb hCKe hCb in
+        let hCg' = lemma_check_substitute_intros mode i rows e (subst1 eg eb) hCKe hCg in
+        Inr (hCb', hCg')
+    in
+
+    CkContract _ ps (subst1' er i e) (subst1' eg (i + 1) (lift1 e a)) (subst1' eb i e) hTr' hTrg' hCr' hCgb'
+
+and lemma_check_substitute_intros_apps
+  (#t: table)
+  (#c: context t)
+  (#a: funty t.ty)
+  (mode: PM.check_mode)
+  (i: C.index_lookup c)
+  (rows: list (row (C.drop1 c i)))
+  (e: exp t (C.drop1 c i) (C.get_index c i) { causal e })
+  (e': exp_apps t c a)
+  (hCKe: (r: list (row (C.drop1 c i)) { List.length r <= List.length rows }) -> check mode r e)
+  (hCKe': check_apps mode (subst_extend_dropped i rows e) e'):
+    Tot (check_apps mode rows (subst1_apps' e' i e)) (decreases hCKe') =
+  match e' with
+  | XPrim f -> CkPrim rows f
+  | XApp ef ea ->
+    let CkApp _ _ _ hCKf hCKa = hCKe' in
+    let hCKf' = lemma_check_substitute_intros_apps mode i rows e ef hCKe hCKf in
+    let hCKa' = lemma_check_substitute_intros mode i rows e ea hCKe hCKa in
+    CkApp rows _ _ hCKf' hCKa'
+
+
+
+let lemma_check_substitute_intros_no_dep_base
+  (#t: table)
+  (#c: context t)
+  (#a: t.ty)
+  (mode: PM.check_mode)
+  (i: C.index_lookup c)
+  (rows: list (row (C.drop1 c i)))
+  (e: exp t (C.drop1 c i) (C.get_index c i) { causal e })
+  (e': exp_base t c a { ~ (direct_dependency_base e' i) }):
+    Tot (check mode rows (subst1_base' e' i e)) =
+  match e' with
+  | XVal v -> CkBase rows (XVal v)
+  | XVar x -> CkBase rows (XVar x)
+  | XBVar i' ->
+    assert (i <> i');
+    if i' < i
+    then (
+      CP.lemma_drop_get_index_lt c i i';
+      let i': C.index_lookup (C.drop1 c i) = i' in
+      let xv: exp_base t (C.drop1 c i) a = XBVar i' in
+      CkBase rows xv
+    ) else (
+      CP.lemma_drop_get_index_gt c i (i' - 1);
+      assert (C.opt_index (C.drop1 c i) (i' - 1) == Some (C.get_index c i'));
+      assert_norm (subst1_base' (XBVar i') i e == XBase (XBVar #t #(C.drop1 c i) (i' - 1)));
+      CkBase rows (XBVar (i' - 1)))
+
+let rec lemma_check_substitute_intros_no_dep
+  (#t: table)
+  (#c: context t)
+  (#a: t.ty)
+  (mode: PM.check_mode)
+  (i: C.index_lookup c)
+  (rows: list (row (C.drop1 c i)))
+  (e: exp t (C.drop1 c i) (C.get_index c i) { causal e })
+  (e': exp t c a { ~ (direct_dependency e' i) })
+  (hCKe: (r: list (row (C.drop1 c i)) { List.length r < List.length rows }) -> check mode r e)
+  (hCKe': check mode (subst_extend_dropped i rows e) e'):
+    Tot (check mode rows (subst1' e' i e)) (decreases hCKe') =
+  match e' with
+  | XBase b ->
+    lemma_check_substitute_intros_no_dep_base mode i rows e b
+
+  | XApps ea ->
+    let CkApps _ _ hCKa = hCKe' in
+    CkApps _ _ (lemma_check_substitute_intros_no_dep_apps mode i rows e ea hCKe hCKa)
+
+  | XFby v1 e2 ->
+    (match hCKe' with
+    | CkFby1 _ _ _ -> CkFby1 rows v1 (subst1' e2 i e)
+    | CkFbyS _ _ _ _ hCK2 ->
+      CkFbyS (List.hd rows) (List.tl rows) v1 (subst1' e2 i e) (lemma_check_substitute_intros mode i (List.tl rows) e e2 hCKe hCK2))
+
+  | XMu e1 ->
+    let CkMu _ _ hCK1 = hCKe' in
+    lemma_subst_subst_distribute_XMu e1 i e;
+    let hCK1' = lemma_check_substitute_intros_no_dep mode i rows e (subst1 e1 (XMu e1)) hCKe hCK1 in
+    CkMu _ (subst1' e1 (i + 1) (lift1 e a)) hCK1'
+
+  | XLet b e1 e2 ->
+    let CkLet _ _ _ hCK = hCKe' in
+    lemma_subst_subst_distribute_le e2 0 i e1 e;
+    let hCK' = lemma_check_substitute_intros_no_dep mode i rows e (subst1 e2 e1) hCKe hCK in
+    CkLet _ (subst1' e1 i e) (subst1' e2 (i + 1) (lift1 e b)) hCK'
+
+  | XCheck ps e1 ->
+    let CkCheck _ _ _ hCK hBS = hCKe' in
+    let hCK' = lemma_check_substitute_intros_no_dep mode i rows e e1 hCKe hCK in
+    lemma_bigstep_always_substitute i rows e e1;
+    CkCheck _ ps (subst1' e1 i e) hCK' ()
+
+  | XContract ps er eg eb ->
+    let CkContract _ _ _ _ _ hTr hTrg hCr hCgb = hCKe' in
+    lemma_bigstep_always_substitute i rows e er;
+    lemma_bigstep_always_substitute i rows e (subst1 eg eb);
+
+    let hTr' = () in
+    let hTrg' = () in
+
+    let hCr' = lemma_check_substitute_intros_no_dep mode i rows e er hCKe hCr in
+
+    let hCgb' = match hCgb with
+      | Inl hN ->
+        Inl ()
+      | Inr (hCb,hCg) ->
+        lemma_subst_subst_distribute_le eg 0 i eb e;
+        let hCb' = lemma_check_substitute_intros_no_dep mode i rows e eb hCKe hCb in
+        let hCg' = lemma_check_substitute_intros_no_dep mode i rows e (subst1 eg eb) hCKe hCg in
+        Inr (hCb', hCg')
+    in
+
+    let hC' = CkContract _ ps (subst1' er i e) (subst1' eg (i + 1) (lift1 e a)) (subst1' eb i e) hTr' hTrg' hCr' hCgb' in
+    admit ()
+
+and lemma_check_substitute_intros_no_dep_apps
+  (#t: table)
+  (#c: context t)
+  (#a: funty t.ty)
+  (mode: PM.check_mode)
+  (i: C.index_lookup c)
+  (rows: list (row (C.drop1 c i)))
+  (e: exp t (C.drop1 c i) (C.get_index c i) { causal e })
+  (e': exp_apps t c a { ~ (direct_dependency_apps e' i) })
+  (hCKe: (r: list (row (C.drop1 c i)) { List.length r < List.length rows }) -> check mode r e)
+  (hCKe': check_apps mode (subst_extend_dropped i rows e) e'):
+    Tot (check_apps mode rows (subst1_apps' e' i e)) (decreases hCKe') =
+  match e' with
+  | XPrim f -> CkPrim rows f
+  | XApp ef ea ->
+    let CkApp _ _ _ hCKf hCKa = hCKe' in
+    let hCKf' = lemma_check_substitute_intros_no_dep_apps mode i rows e ef hCKe hCKf in
+    let hCKa' = lemma_check_substitute_intros_no_dep mode i rows e ea hCKe hCKa in
+    CkApp rows _ _ hCKf' hCKa'
