src/Pipit.System.Exp.Check.Sound.fst
@@ -1,0 +1,123 @@
+module Pipit.System.Exp.Check.Sound
+
+open Pipit.Prim.Table
+open Pipit.Exp.Base
+open Pipit.System.Exp.Check.Base
+
+open FStar.Squash
+
+module SXCA = Pipit.System.Exp.Check.Assumptions
+module SXCO = Pipit.System.Exp.Check.Obligations
+
+module CR  = Pipit.Context.Row
+
+module SB  = Pipit.System.Base
+module SX  = Pipit.System.Exp
+module SXP = Pipit.System.Exp.Properties
+module SI  = Pipit.System.Ind
+
+module XB  = Pipit.Exp.Bigstep
+module XC  = Pipit.Exp.Causality
+module XK  = Pipit.Exp.Checked.Base
+
+module PM = Pipit.Prop.Metadata
+
+module T    = FStar.Tactics
+
+#push-options "--split_queries always"
+
+let check_invariant_all
+  (#t: table) (#c: context t) (#a: t.ty)
+  (mode: PM.check_mode)
+  (e: exp t c a { XC.causal e }):
+    Tot prop =
+  forall (rows: list (row c)).
+    check_invariant rows e mode
+
+
+let checkK_init
+  (#t: table) (#c: context t) (#a: t.ty)
+  (e: exp t c a { XC.causal e })
+  (mode: PM.check_mode):
+  Lemma (ensures (
+    XK.check_prop mode [] e
+  ))
+  // TODO:ADMIT: needs fancy substitution like in Causality?
+  = admit ()
+
+let check_all_Fby
+  (#t: table) (#c: context t) (#a: t.ty)
+  (v: t.ty_sem a)
+  (e: exp t c a { XC.causal e })
+  (mode: PM.check_mode):
+  Lemma
+    (requires (
+      XK.check_all mode (XFby v e)
+    ))
+    (ensures (
+      XK.check_all mode e
+    ))
+  =
+  introduce forall (rows: list (row c)). XK.check_prop mode rows e
+  with
+    match rows with
+    | [] -> checkK_init e mode // check_init e mode
+    | r::_ ->
+      assert (XK.check_prop mode (r::rows) (XFby v e));
+      let hC: squash (XK.check mode (r::rows) (XFby v e)) = () in
+      let hC': squash (XK.check mode rows e) =
+        bind_squash hC (fun hC ->
+        match hC with
+        | XK.CkFbyS _ _ _ _ _ -> ()
+        | _ -> false_elim ()
+      ) in
+      ()
+
+
+let rec check_invariant_of_check_all
+  (#t: table) (#c: context t) (#a: t.ty)
+  (rows: list (row c))
+  (e: exp t c a { XC.causal e })
+  (mode: PM.check_mode):
+  Lemma
+    (requires (
+      XK.check_all mode e
+    ))
+    (ensures (
+      check_invariant rows e mode
+    ))
+    (decreases e)
+    =
+  match e with
+  | XBase _ -> ()
+  | XFby v e1 ->
+    check_all_Fby v e1 mode;
+    check_invariant_of_check_all rows e1 mode
+  | XMu e1 ->
+    admit ()
+  | _ -> admit ()
+
+let rec check_all_of_check_unknown
+  (#t: table) (#c: context t) (#a: t.ty)
+  (rows: list (row c))
+  (e: exp t c a { XC.causal e }):
+  Lemma
+    (requires (
+      XK.check_all PM.check_mode_valid e /\
+      check_invariant_all PM.check_mode_unknown e
+    ))
+    (ensures (
+      XK.check PM.check_mode_unknown rows e
+    ))
+    (decreases e)
+    =
+  match e with
+  | XBase b -> return_squash (XK.CkBase #PM.check_mode_unknown rows b)
+  // | XFby v e1 ->
+  //   check_all_Fby v e1 PM.check_mode_valid;
+  //   check_all_of_check_unknown rows e1
+    // check_invariant_of_check_all rows e1 mode
+  | XMu e1 ->
+    admit ()
+  | _ -> admit ()
+
